proof/crefine/AutoCorresTest.thy
@@ -1,33 +1,13 @@
-(*
- * @LICENSE(NICTA) (FIXME?)
- *)
-
 (* Experimental AutoCorres proofs over CRefine: work in progress *)
 
 theory AutoCorresTest
-imports "../../tools/autocorres/AutoCorres"
-        "../../tools/autocorres/L4VerifiedLinks"
-        AutoCorresModifiesProofs
+imports (* Frameworks and tactics *)
+        AutoCorres_C
         (* import Refine_C last to minimise change to global context *)
         Refine_C
 begin
 
-ML \<open>
-fun do_ac_modifies_rules filename ctxt = let
-    val fn_info = Symtab.lookup (AutoCorresFunctionInfo.get (Proof_Context.theory_of ctxt)) filename |> the;
-    val prog_info = ProgramInfo.get_prog_info ctxt filename;
-    val existing_modifies =
-          Symtab.dest (FunctionInfo.get_functions fn_info)
-          |> List.mapPartial (fn (fn_name, fn_def) =>
-               if not (#finished fn_def) then NONE else
-                 SOME (fn_name, Proof_Context.get_thm ctxt (fn_name ^ "'_modifies")))
-    val all_function_groups = FunctionInfo.get_topo_sorted_functions fn_info;
-    val (callee_modifies, results, ctxt') =
-          fold (AutoCorresModifiesProofs.define_modifies_group fn_info prog_info)
-               all_function_groups (AutoCorresModifiesProofs.build_incr_net (map snd existing_modifies),
-                                    Symtab.make existing_modifies, ctxt)
-in ctxt' end
-\<close>
+section \<open>Simple test case: handleYield\<close>
 
 autocorres
   [
@@ -38,173 +18,16 @@ autocorres
    no_c_termination
   ] "c/kernel_all.c_pp"
 
-(* Prove and store modifies rules. *)
-context kernel_all_substitute begin
-local_setup \<open>do_ac_modifies_rules "c/kernel_all.c_pp"\<close>
-end
-
-
-subsection \<open>Proof frameworks\<close>
-
-
 context kernel_m begin
 
-thm handleYield_body_def
-    handleYield'_def
-    handleYield_def
-    tcbSchedDequeue'_def
-    tcbSchedDequeue'_def[unfolded AC_call_L1_def L2_call_L1_def L1_call_simpl_def]
-thm handleYield'_ac_corres
-thm handleYield'_modifies
-desugar_thm handleYield_modifies[unfolded mex_def meq_def] "may_only"
-
-text \<open>
-  From AutoCorres @{term ac_corres}, obtain @{term ccorres}.
-  This requires a separate corres_underlying proof between the
-  AutoCorres spec and design Spec, in order to establish @{term cstate_relation}.
-\<close>
-lemma autocorres_to_ccorres:
-  "\<lbrakk> ac_corres globals check_termination \<Gamma> ret_xf arg_rel (liftE ac_f) (Call f_'proc);
-     arg_relS = Collect arg_rel;
-     corres_underlying {(s, s'). cstate_relation s s'} True True R P \<top> dspec_f ac_f \<rbrakk> \<Longrightarrow>
-   ccorres dc xfdc P arg_relS [] dspec_f (Call f_'proc)"
-  by (fastforce simp: ccorres_underlying_def corres_underlying_def rf_sr_def Ball_def
-                      liftE_def in_liftE[simplified liftE_def] unif_rrel_def
-                dest: ac_corres_ccorres_underlying split: xstate.splits)
-
-text \<open>
-  From @{term ccorres} obtain @{term corres}.
-  This is for exporting existing ccorres theorems to be used
-  in AutoCorres-based corres proofs.
-\<close>
-thm AC_call_L1_def L2_call_L1_def L1_call_simpl_def
-lemma in_AC_call_simpl:
-  fixes r s s' arg_pred globals ret_xf \<Gamma> f_'proc
-  shows "(r, s') \<in> fst (AC_call_L1 arg_pred globals ret_xf (L1_call_simpl check_termination \<Gamma> f_'proc) s) \<Longrightarrow>
-         \<exists>cs cs'. s = globals cs \<and> arg_pred cs \<and>
-                  (check_termination \<longrightarrow> \<Gamma> \<turnstile> Call f_'proc \<down> Normal cs) \<and>
-                  \<Gamma> \<turnstile> \<langle>Call f_'proc, Normal cs\<rangle> \<Rightarrow> Normal cs' \<and>
-                  s' = globals cs' \<and> r = ret_xf cs'"
-  apply (clarsimp simp: AC_call_L1_def L2_call_L1_def L1_call_simpl_def)
-  apply (monad_eq simp: liftM_def select_def select_f_def liftE_def split: xstate.splits sum.splits)
-  apply (rename_tac cs cs' status)
-  apply (case_tac status)
-  apply auto
-  done
-
-lemma ccorres_to_corres_partial:
-  assumes ac_def: "ac_f \<equiv> AC_call_L1 arg_rel globals ret_xf (L1_call_simpl check_termination \<Gamma> f_'proc)"
-  shows "\<lbrakk> ccorres R ret_xf P (Collect arg_rel) [] dspec_f (Call f_'proc) \<rbrakk> \<Longrightarrow>
-         corres_underlying {(s, s'). cstate_relation s s'} True False R P \<top> dspec_f ac_f"
-  by (fastforce simp: unif_rrel_def ac_def corres_underlying_def ccorres_underlying_def rf_sr_def
-                intro: EHOther dest: in_AC_call_simpl)
-
-text \<open>
-  A fantasy world where ccorres_underlying proves termination.
-\<close>
-context begin
-
-private lemma ccorres_underlying_idealised_def:
-  "ccorres_underlying srel \<Gamma> rrel xf arrel axf G G' hs \<equiv>
-   \<lambda>m c. \<forall>(s, s')\<in>srel.
-            G s \<and> s' \<in> G' \<and> \<not> snd (m s) \<longrightarrow>
-            \<Gamma> \<turnstile> c \<down> Normal s' \<and>
-            (\<forall>n t. \<Gamma>\<turnstile>\<^sub>h \<langle>c # hs,s'\<rangle> \<Rightarrow> (n, t) \<longrightarrow>
-                   (case t of Normal s'' \<Rightarrow> \<exists>(r, t)\<in>fst (m s). (t, s'') \<in> srel \<and> unif_rrel (n = length hs) rrel xf arrel axf r s'' | _ \<Rightarrow> False))"
-  sorry
-
-private lemma ccorres_to_corres_idealised:
-  assumes ac_def: "ac_f \<equiv> AC_call_L1 arg_rel globals ret_xf (L1_call_simpl check_termination \<Gamma> f_'proc)"
-  shows "\<lbrakk> ccorres R ret_xf P (Collect arg_rel) [] dspec_f (Call f_'proc) \<rbrakk> \<Longrightarrow>
-         corres_underlying {(s, s'). cstate_relation s s'} True True R P \<top> dspec_f ac_f"
-  apply (clarsimp simp: ac_def corres_underlying_def ccorres_underlying_def rf_sr_def Ball_def Bex_def)
-  apply (rule conjI)
-   -- "proof for return values"
-   apply (fastforce simp: unif_rrel_def intro: EHOther dest: in_AC_call_simpl)
-
-  -- "proof for fail bit is trickier"
-  apply (clarsimp simp: AC_call_L1_def L2_call_L1_def L1_call_simpl_def)
-  apply (case_tac check_termination)
-   apply (clarsimp simp: select_f_def select_def snd_bind split: sum.splits prod.splits)
-   apply (clarsimp simp: Bex_def get_def)
-   apply (erule impE)
-    -- "oops... @{term ccorres} doesn't give us @{term terminates}"
-    subgoal sorry
-   apply (erule disjE)
-    apply (monad_eq split: xstate.splits sum.splits)
-     apply (drule EHOther, fastforce)
-     apply blast
-    apply (drule EHOther, fastforce)
-    apply blast
-   apply (monad_eq split: xstate.splits)
-   apply (fastforce dest: EHAbrupt[OF _ EHEmpty])
-
-  (* FIXME: duplication *)
-  apply (clarsimp simp: select_f_def select_def snd_bind split: sum.splits prod.splits)
-  apply (clarsimp simp: Bex_def get_def)
-  apply (erule disjE)
-   apply (monad_eq split: xstate.splits sum.splits)
-    apply (drule EHOther, fastforce)
-    apply blast
-   apply (drule EHOther, fastforce)
-   apply blast
-  apply (monad_eq split: xstate.splits)
-  apply (fastforce dest: EHAbrupt[OF _ EHEmpty])
-  done
-
-text \<open>With proposed alternative ccorres...\<close>
-private lemma
-  assumes ac_def: "ac_f \<equiv> AC_call_L1 arg_rel globals ret_xf (L1_call_simpl check_termination \<Gamma> f_'proc)"
-  shows "\<lbrakk> ccorres R ret_xf P (Collect arg_rel) [] dspec_f (Call f_'proc) \<rbrakk> \<Longrightarrow>
-         corres_underlying {(s, s'). cstate_relation s s'} True True R P \<top> dspec_f ac_f"
-  apply (clarsimp simp: ac_def corres_underlying_def ccorres_underlying_idealised_def rf_sr_def Ball_def Bex_def)
-  apply (rule conjI)
-   -- "proof for return values"
-   apply (fastforce simp: unif_rrel_def intro: EHOther dest: in_AC_call_simpl)
-
-  -- "proof for fail bit is trickier"
-  apply (clarsimp simp: AC_call_L1_def L2_call_L1_def L1_call_simpl_def)
-  apply (clarsimp simp: select_f_def select_def snd_bind split: sum.splits prod.splits)
-  apply (clarsimp simp: Bex_def get_def)
-  apply (erule disjE)
-   apply (monad_eq split: xstate.splits sum.splits)
-    apply (drule EHOther, fastforce)
-    apply blast
-   apply (drule EHOther, fastforce)
-   apply blast
-  apply (monad_eq split: xstate.splits)
-  apply (fastforce dest: EHAbrupt[OF _ EHEmpty])
-  done
-
-
-lemma ccorres_rrel_nat_unit:
-  "ccorres op = (\<lambda>s. ()) st_P arg_P hs m c = ccorres dc xfdc st_P arg_P hs m c"
-  by (simp add: ccorres_underlying_def dc_def xfdc_def unif_rrel_def cong del: xstate.case_cong)
-
-
-
-subsection \<open>Case study: handleYield\<close>
-
-(* AutoCorres translation of handleYield *)
-thm handleYield'_def
-
-(* handleYield calls un-translated functions, such as tcbSchedDequeue *)
-thm tcbSchedDequeue_body_def
-(* AutoCorres produces a monadic wrapper of the SIMPL code *)
-thm tcbSchedDequeue'_def
-    tcbSchedDequeue'_def[unfolded AC_call_L1_def L2_call_L1_def L1_call_simpl_def]
-
-
-text \<open>
-  First, create some corres versions of ccorres rules.
-\<close>
+text \<open>Export corres_underlying rules for handleYield's callees.\<close>
 thm getCurThread_ccorres
-lemma getCurThread_corres:
+lemma getCurThread_wrapper_corres:
   "corres_underlying {(x, y). cstate_relation x y} True True (\<lambda>ct ct'. tcb_ptr_to_ctcb_ptr ct = ct') invs' (\<lambda>_. True) getCurThread (gets ksCurThread_')"
   by (simp add: getCurThread_def cstate_relation_def Let_def)
 
 thm ccorres_pre_getCurThread
-lemma corres_pre_getCurThread:
+lemma corres_pre_getCurThread_wrapper:
   assumes cc: "\<And>rv rv'. rv' = tcb_ptr_to_ctcb_ptr rv \<Longrightarrow>
                   corres_underlying {(x, y). cstate_relation x y} True True R (P rv) (P' rv) (f rv) (f' rv')"
   shows   "corres_underlying {(x, y). cstate_relation x y} True True R
@@ -219,246 +42,7 @@ lemma corres_pre_getCurThread:
   done
 
 thm tcbSchedDequeue_ccorres
-private lemma tcbSchedDequeue_corres_cheat:
-  "tcb_ptr_to_ctcb_ptr ct = ct' \<Longrightarrow>
-   corres_underlying {(x, y). cstate_relation x y} True True (op=)
-     (Invariants_H.valid_queues and valid_queues' and tcb_at' ct and valid_objs') \<top>
-     (tcbSchedDequeue ct) (tcbSchedDequeue' ct')"
-  apply (rule ccorres_to_corres_idealised)
-   apply (simp add: tcbSchedDequeue'_def)
-  apply (clarsimp simp: ccorres_rrel_nat_unit tcbSchedDequeue_ccorres[simplified])
-  done
-
-thm tcbSchedAppend_ccorres
-private lemma tcbSchedAppend_corres_cheat:
-  "tcb_ptr_to_ctcb_ptr ct = ct' \<Longrightarrow>
-   corres_underlying {(x, y). cstate_relation x y} True True (op=)
-     (Invariants_H.valid_queues and tcb_at' ct and valid_objs') \<top>
-     (tcbSchedAppend ct) (tcbSchedAppend' ct')"
-  apply (rule ccorres_to_corres_idealised)
-   apply (simp add: tcbSchedAppend'_def)
-  apply (clarsimp simp: ccorres_rrel_nat_unit tcbSchedAppend_ccorres[simplified])
-  done
-
-thm rescheduleRequired_ccorres
-private lemma rescheduleRequired_corres_cheat:
-  "corres_underlying {(x, y). cstate_relation x y} True True (op=)
-     (Invariants_H.valid_queues and (\<lambda>s. weak_sch_act_wf (ksSchedulerAction s) s) and valid_objs') \<top>
-     rescheduleRequired rescheduleRequired'"
-  apply (rule ccorres_to_corres_idealised)
-   apply (simp add: rescheduleRequired'_def)
-  apply (clarsimp simp: ccorres_rrel_nat_unit rescheduleRequired_ccorres[simplified])
-  done
-
-text \<open>Returning to the real world...\<close>
-end
-
-
-
-subsection \<open>Termination on demand\<close>
-text \<open>
-  Instead of adding termination to ccorres in one go,
-  we can also prove terminates as incremental side conditions.
-
-  To begin with, we can automatically prove terminates for most
-  helper functions as they do not have recursion or loops.
-\<close>
-
-named_theorems terminates_trivial
-
-lemma [terminates_trivial]:
-  "\<lbrakk> \<And>s. \<Gamma> \<turnstile> c \<down> Normal s \<rbrakk> \<Longrightarrow> \<Gamma> \<turnstile> Guard F G c \<down> Normal s"
-  apply (blast intro: terminates.Guard terminates.GuardFault)
-  done
-lemma [terminates_trivial]:
-  "\<lbrakk> \<And>s. \<Gamma> \<turnstile> c1 \<down> Normal s; \<And>s. \<Gamma> \<turnstile> c2 \<down> Normal s \<rbrakk> \<Longrightarrow>
-   \<Gamma> \<turnstile> Cond C c1 c2 \<down> Normal s"
-  apply (blast intro: terminates.CondTrue terminates.CondFalse)
-  done
-lemma [terminates_trivial]:
-  "\<lbrakk> \<Gamma> \<turnstile> c1 \<down> Normal s; \<And>s. \<Gamma> \<turnstile> c2 \<down> Normal s \<rbrakk> \<Longrightarrow>
-   \<Gamma> \<turnstile> c1;;c2 \<down> Normal s"
-  apply (erule terminates.Seq)
-  apply clarsimp
-  apply (case_tac s'; auto)
-  done
-
-lemma [terminates_trivial]:
-  fixes \<Gamma> return init shows
-  "\<lbrakk> \<And>s. \<Gamma> \<turnstile> Call p \<down> Normal s; \<And>s t u. \<Gamma> \<turnstile> c s t \<down> Normal u \<rbrakk> \<Longrightarrow>
-   \<Gamma> \<turnstile> call init p return c \<down> Normal s"
-  apply (case_tac "\<Gamma> p")
-   apply (erule terminates_callUndefined)
-  apply (fastforce simp: terminates_Call_body intro: terminates_call)
-  done
-
-lemmas [terminates_trivial] =
-  terminates.Basic
-  terminates.Catch[rule_format]
-  terminates.Throw
-  terminates.Skip
-  terminates.Spec
-
-lemma cap_get_capType_terminates:
-  "\<Gamma> \<turnstile> Call cap_get_capType_'proc \<down> Normal s"
-  apply (rule terminates.Call)
-   apply (rule cap_get_capType_impl)
-  apply (unfold cap_get_capType_body_def return_C_def lvar_nondet_init_def)
-  apply (intro terminates_trivial)
-  done
-
-lemma thread_state_get_tcbQueued_terminates:
-  "\<Gamma> \<turnstile> Call thread_state_get_tcbQueued_'proc \<down> Normal s"
-  apply (rule terminates.Call)
-   apply (rule thread_state_get_tcbQueued_impl)
-  apply (unfold thread_state_get_tcbQueued_body_def return_C_def lvar_nondet_init_def)
-  apply (intro terminates_trivial)
-  done
-
-lemma thread_state_ptr_set_tcbQueued_terminates:
-  "\<Gamma> \<turnstile> Call thread_state_ptr_set_tcbQueued_'proc \<down> Normal s"
-  apply (rule terminates.Call)
-   apply (rule thread_state_ptr_set_tcbQueued_impl)
-  apply (unfold thread_state_ptr_set_tcbQueued_body_def return_C_def lvar_nondet_init_def)
-  apply (intro terminates_trivial)
-  done
-
-lemma ready_queues_index_terminates:
-  "\<Gamma> \<turnstile> Call ready_queues_index_'proc \<down> Normal s"
-  apply (rule terminates.Call)
-   apply (rule ready_queues_index_impl)
-  apply (unfold ready_queues_index_body_def return_C_def lvar_nondet_init_def)
-  apply (intro terminates_trivial)
-  done
-
-lemma prio_to_l1index_terminates:
-  "\<Gamma> \<turnstile> Call prio_to_l1index_'proc \<down> Normal s"
-  apply (rule terminates.Call)
-   apply (rule prio_to_l1index_impl)
-  apply (unfold prio_to_l1index_body_def return_C_def lvar_nondet_init_def)
-  apply (intro terminates_trivial)
-  done
-
-lemma removeFromBitmap_terminates:
-  "\<Gamma> \<turnstile> Call removeFromBitmap_'proc \<down> Normal s"
-  apply (rule terminates.Call)
-   apply (rule removeFromBitmap_impl)
-  apply (unfold removeFromBitmap_body_def return_C_def lvar_nondet_init_def)
-  apply (intro terminates_trivial prio_to_l1index_terminates)
-  done
-
-lemma addToBitmap_terminates:
-  "\<Gamma> \<turnstile> Call addToBitmap_'proc \<down> Normal s"
-  apply (rule terminates.Call)
-   apply (rule addToBitmap_impl)
-  apply (unfold addToBitmap_body_def return_C_def lvar_nondet_init_def)
-  apply (intro terminates_trivial prio_to_l1index_terminates)
-  done
-
-lemma tcbSchedDequeue_terminates:
-   "\<Gamma> \<turnstile> Call tcbSchedDequeue_'proc \<down> Normal s"
-  apply (rule terminates.Call)
-   apply (rule tcbSchedDequeue_impl)
-  apply (unfold tcbSchedDequeue_body_def return_C_def lvar_nondet_init_def)
-  apply (intro terminates_trivial
-          thread_state_get_tcbQueued_terminates
-          thread_state_ptr_set_tcbQueued_terminates
-          ready_queues_index_terminates
-          removeFromBitmap_terminates)
-  done
-
-lemma tcbSchedAppend_terminates:
-   "\<Gamma> \<turnstile> Call tcbSchedAppend_'proc \<down> Normal s"
-  apply (rule terminates.Call)
-   apply (rule tcbSchedAppend_impl)
-  apply (unfold tcbSchedAppend_body_def return_C_def lvar_nondet_init_def)
-  apply (intro terminates_trivial
-          thread_state_get_tcbQueued_terminates
-          thread_state_ptr_set_tcbQueued_terminates
-          ready_queues_index_terminates
-          addToBitmap_terminates)
-  done
-
-lemma tcbSchedEnqueue_terminates:
-   "\<Gamma> \<turnstile> Call tcbSchedEnqueue_'proc \<down> Normal s"
-  apply (rule terminates.Call)
-   apply (rule tcbSchedEnqueue_impl)
-  apply (unfold tcbSchedEnqueue_body_def return_C_def lvar_nondet_init_def)
-  apply (intro terminates_trivial
-          thread_state_get_tcbQueued_terminates
-          thread_state_ptr_set_tcbQueued_terminates
-          ready_queues_index_terminates
-          addToBitmap_terminates)
-  done
-
-lemma rescheduleRequired_terminates:
-   "\<Gamma> \<turnstile> Call rescheduleRequired_'proc \<down> Normal s"
-  apply (rule terminates.Call)
-   apply (rule rescheduleRequired_impl)
-  apply (unfold rescheduleRequired_body_def return_C_def lvar_nondet_init_def)
-  apply (intro terminates_trivial
-          tcbSchedEnqueue_terminates)
-  done
-
-
-text \<open>Process handleYield's callees without cheating\<close>
-
-text \<open>Requires termination proof for f_'proc. Used when no_c_termination is off.\<close>
-lemma ccorres_to_corres_with_termination:
-  assumes ac_def: "ac_f \<equiv> AC_call_L1 arg_rel globals ret_xf (L1_call_simpl True \<Gamma> f_'proc)"
-  assumes terminates:
-    "\<And>s s'. \<lbrakk> cstate_relation s (globals s'); P s; \<not> snd (dspec_f s); arg_rel s' \<rbrakk> \<Longrightarrow>
-            \<Gamma> \<turnstile> Call f_'proc \<down> Normal s'"
-  shows "\<lbrakk> ccorres R ret_xf P (Collect arg_rel) [] dspec_f (Call f_'proc) \<rbrakk> \<Longrightarrow>
-         corres_underlying {(s, s'). cstate_relation s s'} True True R P \<top> dspec_f ac_f"
-  apply (clarsimp simp: ac_def corres_underlying_def ccorres_underlying_def rf_sr_def Ball_def Bex_def)
-  apply (rule conjI)
-   -- "proof for return values"
-   apply (fastforce simp: unif_rrel_def intro: EHOther dest: in_AC_call_simpl)
-
-  -- "proof for fail bit is trickier"
-  apply (clarsimp simp: AC_call_L1_def L2_call_L1_def L1_call_simpl_def)
-  apply (clarsimp simp: select_f_def select_def snd_bind split: sum.splits prod.splits)
-  apply (clarsimp simp: Bex_def get_def)
-  apply (erule impE)
-   apply (blast intro: terminates)
-  apply (erule disjE)
-   apply (monad_eq split: xstate.splits sum.splits)
-    apply (drule EHOther, fastforce)
-    apply blast
-   apply (drule EHOther, fastforce)
-   apply blast
-  apply (monad_eq split: xstate.splits)
-  apply (fastforce dest: EHAbrupt[OF _ EHEmpty])
-  done
-
-text \<open>Does not require termination proof for f_'proc. Used with no_c_termination.\<close>
-lemma ccorres_to_corres_no_termination:
-  assumes ac_def: "ac_f \<equiv> AC_call_L1 arg_rel globals ret_xf (L1_call_simpl False \<Gamma> f_'proc)"
-  shows "\<lbrakk> ccorres R ret_xf P (Collect arg_rel) [] dspec_f (Call f_'proc) \<rbrakk> \<Longrightarrow>
-         corres_underlying {(s, s'). cstate_relation s s'} True True R P \<top> dspec_f ac_f"
-  apply (clarsimp simp: ac_def corres_underlying_def ccorres_underlying_def rf_sr_def Ball_def Bex_def)
-  apply (rule conjI)
-   -- "proof for return values"
-   apply (fastforce simp: unif_rrel_def intro: EHOther dest: in_AC_call_simpl)
-
-  -- "proof for fail bit is trickier"
-  apply (clarsimp simp: AC_call_L1_def L2_call_L1_def L1_call_simpl_def)
-  apply (clarsimp simp: select_f_def select_def snd_bind split: sum.splits prod.splits)
-  apply (clarsimp simp: Bex_def get_def)
-  apply (erule disjE)
-   apply (monad_eq split: xstate.splits sum.splits)
-    apply (drule EHOther, fastforce)
-    apply blast
-   apply (drule EHOther, fastforce)
-   apply blast
-  apply (monad_eq split: xstate.splits)
-  apply (fastforce dest: EHAbrupt[OF _ EHEmpty])
-  done
-
-
-thm tcbSchedDequeue_ccorres
-lemma tcbSchedDequeue_corres:
+lemma tcbSchedDequeue_wrapper_corres:
   "tcb_ptr_to_ctcb_ptr ct = ct' \<Longrightarrow>
    corres_underlying {(x, y). cstate_relation x y} True True (op=)
      (Invariants_H.valid_queues and valid_queues' and tcb_at' ct and valid_objs') \<top>
@@ -469,7 +53,7 @@ lemma tcbSchedDequeue_corres:
   done
 
 thm tcbSchedAppend_ccorres
-lemma tcbSchedAppend_corres:
+lemma tcbSchedAppend_wrapper_corres:
   "tcb_ptr_to_ctcb_ptr ct = ct' \<Longrightarrow>
    corres_underlying {(x, y). cstate_relation x y} True True (op=)
      (Invariants_H.valid_queues and tcb_at' ct and valid_objs') \<top>
@@ -480,7 +64,7 @@ lemma tcbSchedAppend_corres:
   done
 
 thm rescheduleRequired_ccorres
-lemma rescheduleRequired_corres:
+lemma rescheduleRequired_wrapper_corres:
   "corres_underlying {(x, y). cstate_relation x y} True True (op=)
      (Invariants_H.valid_queues and (\<lambda>s. weak_sch_act_wf (ksSchedulerAction s) s) and valid_objs') \<top>
      rescheduleRequired rescheduleRequired'"
@@ -494,10 +78,11 @@ text \<open>
   The handleYield spec has one less getCurThread, so we need to use the fact
   that tcbSchedDequeue does not modify ksCurThread.
 \<close>
+local_setup \<open>AutoCorresModifiesProofs.new_modifies_rules "c/kernel_all.c_pp"\<close>
 thm tcbSchedDequeue'_modifies
 
 text \<open>Existing ccorres proof, for reference\<close>
-lemma
+lemma (* handleYield_ccorres: *)
   "ccorres dc xfdc
        (invs' and ct_active')
        UNIV
@@ -530,9 +115,15 @@ lemma reorder_gets:
 
 text \<open>Now the proof.\<close>
 lemma (* handleYield_ccorres: *)
-  "ccorres dc xfdc (invs' and ct_active') UNIV [] handleYield (Call handleYield_'proc)"
-  apply (rule autocorres_to_ccorres[OF _ refl, where arg_rel = \<top>, simplified Collect_True])
-   apply (rule kernel_all_substitute.handleYield'_ac_corres)
+  "ccorres dc xfdc
+       (invs' and ct_active')
+       UNIV
+       []
+       (handleYield)
+       (Call handleYield_'proc)"
+  apply (rule ac_corres_to_ccorres)
+    apply (rule kernel_all_substitute.handleYield'_ac_corres)
+   apply simp
   apply (simp add: handleYield_def handleYield'_def)
 
   apply (rule corres_guard_imp)
@@ -542,10 +133,10 @@ lemma (* handleYield_ccorres: *)
      using tcbSchedDequeue'_modifies apply (fastforce simp: valid_def)
     apply (subst gets_gets)
 
-    apply (rule corres_pre_getCurThread)
-    apply (rule corres_split[OF _ tcbSchedDequeue_corres])
-       apply (rule corres_split[OF _ tcbSchedAppend_corres])
-          apply (rule rescheduleRequired_corres)
+    apply (rule corres_pre_getCurThread_wrapper)
+    apply (rule corres_split[OF _ tcbSchedDequeue_wrapper_corres])
+       apply (rule corres_split[OF _ tcbSchedAppend_wrapper_corres])
+          apply (rule rescheduleRequired_wrapper_corres)
          apply (solves simp)
         apply (solves \<open>wp tcbSchedAppend_valid_objs' weak_sch_act_wf_lift_linear | simp\<close>)+
      apply (solves \<open>wp tcbSchedDequeue_invs' tcbSchedDequeue_typ_at'
@@ -560,36 +151,8 @@ lemma (* handleYield_ccorres: *)
 
 end
 
-context kernel_m begin
-ML \<open>
-(* Search for function call testcase:
- *   function calls with the smallest caller + callee *)
-let val ctxt = @{context};
-    val fn_info = FunctionInfo.init_fn_info ctxt "c/kernel_all.c_pp";
-    val real_funcs =
-          Symtab.dest (FunctionInfo.get_functions fn_info)
-          |> filter (fn (f, info) => case Thm.prop_of (#definition info) of
-                        @{term_pat "_ \<equiv> Spec _"} => false
-                      | @{term_pat "_ \<equiv> TRY SKIP CATCH SKIP END"} => false
-                      | _ => true)
-          |> map fst
-          |> filter (fn f => isSome (try (Proof_Context.get_thm ctxt) (f ^ "_ccorres")))
-          |> Symset.make;
-    val call2s = Symtab.dest (FunctionInfo.get_functions fn_info)
-          |> maps (fn (fn_name, fn_def) =>
-                if not (Symset.contains real_funcs fn_name) then [] else
-                FunctionInfo.get_function_callees fn_info fn_name
-                |> filter (Symset.contains real_funcs)
-                |> map (fn callee =>
-                    (size_of_thm (#definition fn_def) +
-                       size_of_thm (#definition (FunctionInfo.get_function_def fn_info callee)),
-                     (fn_name, callee))));
-in sort (prod_ord int_ord (K EQUAL)) call2s end
-\<close>
-thm handleFault_body_def handleDoubleFault_body_def
-thm handleFault_ccorres handleDoubleFault_ccorres
-end
 
+section \<open>Function call testcase: handleFault and handleDoubleFault\<close>
 
 autocorres
   [
@@ -600,34 +163,12 @@ autocorres
    no_c_termination
   ] "c/kernel_all.c_pp"
 
-(* Prove and store modifies rules. *)
-context kernel_all_substitute begin
-local_setup \<open>do_ac_modifies_rules "c/kernel_all.c_pp"\<close>
-end
-
 context kernel_m begin
-lemma (*handleDoubleFault_ccorres:*)
-  "ccorres dc xfdc (invs' and  tcb_at' tptr and (\<lambda>s. weak_sch_act_wf (ksSchedulerAction s) s) and
-        sch_act_not tptr and (\<lambda>s. \<forall>p. tptr \<notin> set (ksReadyQueues s p)))
-      (UNIV \<inter> {s. tptr_' s = tcb_ptr_to_ctcb_ptr tptr})
-      [] (handleDoubleFault tptr ex1 ex2)
-         (Call handleDoubleFault_'proc)"
-  apply (cinit lift: tptr_')
-   apply (subst ccorres_seq_skip'[symmetric])
-   apply (ctac (no_vcg))
-    apply (rule ccorres_symb_exec_l)
-       apply (rule ccorres_return_Skip)
-      apply (wp asUser_inv getRestartPC_inv)
-    apply (rule empty_fail_asUser)
-    apply (simp add: getRestartPC_def)
-   apply wp
-  apply clarsimp
-  apply (simp add: ThreadState_Inactive_def)
-  apply (fastforce simp: valid_tcb_state'_def)
-  done
+local_setup \<open>AutoCorresModifiesProofs.new_modifies_rules "c/kernel_all.c_pp"\<close>
 
+text \<open>Export corres_underlying rules for handleDoubleFault's callees.\<close>
 thm setThreadState_ccorres[no_vars]
-lemma setThreadState_corres:
+lemma setThreadState_wrapper_corres:
   "(\<forall>cl fl. cthread_state_relation_lifted st (cl\<lparr>tsType_CL := ts && mask 4\<rparr>, fl)) \<and>
    tptr = tcb_ptr_to_ctcb_ptr thread \<Longrightarrow>
    corres_underlying {(x, y). cstate_relation x y} True True (op=)
@@ -644,6 +185,7 @@ lemma setThreadState_corres:
   apply (fastforce simp: ccorres_underlying_def Ball_def)
   done
 
+text \<open>Extra corres_underlying rules.\<close>
 lemma corres_gen_asm':
   "\<lbrakk> corres_underlying sr nf nf' r Q P' f g; \<And>s s'. \<lbrakk> (s, s') \<in> sr; P s; P' s' \<rbrakk> \<Longrightarrow> Q s\<rbrakk> \<Longrightarrow>
    corres_underlying sr nf nf' r P P' f g"
@@ -654,7 +196,7 @@ lemma corres_add_noop_rhs2:
       \<Longrightarrow> corres_underlying sr nf nf' r P P' f g"
   by simp
 
-(* use termination (nf=True) to avoid exs_valid *)
+(* Use termination (nf=True) to avoid exs_valid *)
 lemma corres_noop2_no_exs:
   assumes x: "\<And>s. P s  \<Longrightarrow> \<lbrace>op = s\<rbrace> f \<lbrace>\<lambda>r. op = s\<rbrace> \<and> empty_fail f"
   assumes y: "\<And>s. P' s \<Longrightarrow> \<lbrace>op = s\<rbrace> g \<lbrace>\<lambda>r. op = s\<rbrace>"
@@ -688,13 +230,35 @@ lemma corres_symb_exec_l_no_exs:
    apply simp+
   done
 
-lemma (*handleDoubleFault_ccorres:*)
+text \<open>Existing ccorres proof, for reference\<close>
+lemma (* handleDoubleFault_ccorres: *)
+  "ccorres dc xfdc (invs' and  tcb_at' tptr and (\<lambda>s. weak_sch_act_wf (ksSchedulerAction s) s) and
+        sch_act_not tptr and (\<lambda>s. \<forall>p. tptr \<notin> set (ksReadyQueues s p)))
+      (UNIV \<inter> {s. tptr_' s = tcb_ptr_to_ctcb_ptr tptr})
+      [] (handleDoubleFault tptr ex1 ex2)
+         (Call handleDoubleFault_'proc)"
+  apply (cinit lift: tptr_')
+   apply (subst ccorres_seq_skip'[symmetric])
+   apply (ctac (no_vcg))
+    apply (rule ccorres_symb_exec_l)
+       apply (rule ccorres_return_Skip)
+      apply (wp asUser_inv getRestartPC_inv)
+    apply (rule empty_fail_asUser)
+    apply (simp add: getRestartPC_def)
+   apply wp
+  apply clarsimp
+  apply (simp add: ThreadState_Inactive_def)
+  apply (fastforce simp: valid_tcb_state'_def)
+  done
+
+text \<open>New proof of handleDoubleFault\<close>
+lemma (* handleDoubleFault_ccorres: *)
   "ccorres dc xfdc (invs' and tcb_at' tptr and (\<lambda>s. weak_sch_act_wf (ksSchedulerAction s) s) and
         sch_act_not tptr and (\<lambda>s. \<forall>p. tptr \<notin> set (ksReadyQueues s p)))
       (UNIV \<inter> {s. ex1_' s = ex1' \<and> tptr_' s = tcb_ptr_to_ctcb_ptr tptr})
       [] (handleDoubleFault tptr ex1 ex2)
          (Call handleDoubleFault_'proc)"
-  apply (rule autocorres_to_ccorres[where R="op="])
+  apply (rule ac_corres_to_ccorres[where R="op="])
     apply (rule handleDoubleFault'_ac_corres)
    apply (simp add: pred_conj_def)
   apply (unfold handleDoubleFault_def handleDoubleFault'_def)
@@ -703,7 +267,7 @@ lemma (*handleDoubleFault_ccorres:*)
   apply (rule corres_split')
      (* call setThreadState *)
      apply (rule corres_gen_asm')
-      apply (rule setThreadState_corres)
+      apply (rule setThreadState_wrapper_corres)
       apply (simp add: ThreadState_Inactive_def)
      apply (fastforce simp: valid_tcb_state'_def ThreadState_Inactive_def)
     (* extra haskell code *)
@@ -732,12 +296,10 @@ autocorres
   ] "c/kernel_all.c_pp"
 
 (* Prove and store modifies rules. *)
-context kernel_all_substitute begin
-local_setup \<open>do_ac_modifies_rules "c/kernel_all.c_pp"\<close>
-end
-
 context kernel_m begin
+local_setup \<open>AutoCorresModifiesProofs.new_modifies_rules "c/kernel_all.c_pp"\<close>
 
+(* TODO: proof for handleFault' *)
 thm handleFault_ccorres
 
 end
@@ -745,7 +307,7 @@ end
 
 
 
-
+section \<open>Experiment: translating clzl\<close>
 text \<open>
   __builtin_clzl is defined using guarded_spec_body,
   which is a bit hard to translate generically.
@@ -777,6 +339,7 @@ definition l2_clzl' :: "nat \<Rightarrow> 32 word \<Rightarrow> (globals, unit +
 lemma l2_clzl'_corres:
   "L2corres globals ret__long_' (\<lambda>_. ()) (\<lambda>s. x_' s = x) (l2_clzl' rec_measure' x) (l1_clzl' rec_measure')"
   apply (unfold l2_clzl'_def l1_clzl'_def)
+  (* TODO: how to automate this? *)
   apply (monad_eq simp: L1_defs L2_defs L2corres_def corresXF_def meq_def)
   apply (subst myvars.splits)
   apply simp
@@ -839,7 +402,7 @@ in
 end
 *}
 
-text \<open>Now AutoCorres will use our manual specification in clzl calls.\<close>
+text \<open>Now AutoCorres will use our specification in calls to clzl.\<close>
 autocorres
   [
    skip_heap_abs, skip_word_abs, (* for compatibility *)
@@ -850,7 +413,8 @@ autocorres
   ] "c/kernel_all.c_pp"
 
 context kernel_m begin
-thm clzl'_def chooseThread'_def
+thm clzl'_def
+thm chooseThread'_def
 end
 
 
@@ -883,6 +447,11 @@ end
 
 
 subsection \<open>Experiment with proving bitfield specs\<close>
+
+text \<open>
+  Here we translate some bitfield functions, then separately prove that
+  the translated functions satisfy the bitfield_gen specs.
+\<close>
 autocorres
   [
    skip_heap_abs, skip_word_abs, ts_rules = nondet, (* for compatibility *)
@@ -894,10 +463,6 @@ autocorres
    c_locale = kernel_all_substitute
   ] "c/kernel_all.c_pp"
 
-thm kernel_all_substitute.cap_capType_equals_spec
-thm kernel_all_substitute.cap_capType_equals'_def
-    kernel_all_substitute.cap_capType_equals_body_def
-
 lemma of_bl_from_cond:
   "(if C then 1 else 0) = of_bl [C]"
   by (simp add: word_1_bl)
@@ -905,96 +470,40 @@ lemma of_bl_cond:
   "(if C then of_bl [A] else of_bl [B]) = of_bl [if C then A else B]"
   by (rule if_f)
 
-thm kernel_all_substitute.cap_get_capType'_def[
-      simplified of_bl_from_cond of_bl_cond,
-      folded cap_get_tag_def[simplified mask_def, simplified]]
-thm kernel_all_substitute.cap_cnode_cap_get_capCNodePtr'_def
-thm kernel_all_substitute.cap_cnode_cap_get_capCNodePtr_spec
-thm cap_cnode_cap_lift_def cap_lift_def
-
 context kernel_m begin
-lemma "\<lbrace>\<lambda>_. cap_get_tag cap = scast cap_cnode_cap\<rbrace> cap_cnode_cap_get_capCNodePtr' cap \<lbrace>\<lambda>r _. r = capCNodePtr_CL (cap_cnode_cap_lift cap)\<rbrace>"
+lemma "\<lbrace>\<lambda>_. cap_get_tag cap = scast cap_cnode_cap\<rbrace>
+         cap_cnode_cap_get_capCNodePtr' cap
+       \<lbrace>\<lambda>r _. r = capCNodePtr_CL (cap_cnode_cap_lift cap)\<rbrace>!"
   apply (unfold cap_cnode_cap_get_capCNodePtr'_def)
   apply wp
   apply (simp add: cap_get_tag_def cap_cnode_cap_lift_def cap_lift_def cap_tag_values shiftr_over_and_dist)
   done
 
-lemma "\<lbrace>\<lambda>_. cap_get_tag cap = scast cap_cnode_cap\<rbrace> cap_cnode_cap_get_capCNodeGuard' cap \<lbrace>\<lambda>r _. r = capCNodeGuard_CL (cap_cnode_cap_lift cap)\<rbrace>"
+lemma "\<lbrace>\<lambda>_. cap_get_tag cap = scast cap_cnode_cap\<rbrace>
+         cap_cnode_cap_get_capCNodeGuard' cap
+       \<lbrace>\<lambda>r _. r = capCNodeGuard_CL (cap_cnode_cap_lift cap)\<rbrace>!"
   apply (unfold cap_cnode_cap_get_capCNodeGuard'_def)
   apply wp
   apply (simp add: cap_get_tag_def cap_cnode_cap_lift_def cap_lift_def cap_tag_values shiftr_over_and_dist)
   done
 
-lemma "\<lbrace>\<lambda>_. cap_get_tag cap = scast cap_cnode_cap\<rbrace> cap_cnode_cap_get_capCNodeRadix' cap \<lbrace>\<lambda>r _. r = capCNodeRadix_CL (cap_cnode_cap_lift cap)\<rbrace>"
+lemma "\<lbrace>\<lambda>_. cap_get_tag cap = scast cap_cnode_cap\<rbrace>
+         cap_cnode_cap_get_capCNodeRadix' cap
+       \<lbrace>\<lambda>r _. r = capCNodeRadix_CL (cap_cnode_cap_lift cap)\<rbrace>!"
   apply (unfold cap_cnode_cap_get_capCNodeRadix'_def)
   apply wp
   apply (simp add: cap_get_tag_def cap_cnode_cap_lift_def cap_lift_def cap_tag_values shiftr_over_and_dist)
   done
-
-thm cap_cnode_cap_get_capCNodeRadix'_ac_corres
-thm cap_cnode_cap_get_capCNodeRadix_spec
-thm cap_cnode_cap_get_capCNodeRadix_modifies
 
 end
 
 
 subsection \<open>Experiment with transferring bitfield specs\<close>
 
-text \<open>Generic transfer rules\<close>
-lemma autocorres_transfer_spec:
-  assumes ac_def:
-    "ac_f \<equiv> AC_call_L1 arg_rel globals ret_xf (L1_call_simpl check_termination \<Gamma> f_'proc)"
-  assumes c_spec:
-    "\<forall>s0. \<Gamma>\<turnstile> (Collect (\<lambda>s. s0 = s \<and> P s)) Call f_'proc (Collect (Q s0))"
-  assumes precond_deps:
-    "\<And>s t. \<lbrakk> arg_rel s; arg_rel t; globals s = globals t \<rbrakk> \<Longrightarrow> P s = P t"
-  assumes postcond_deps:
-    "\<And>s0 s0' s t. \<lbrakk> arg_rel s0; arg_rel s0'; globals s0 = globals s0';
-                    ret_xf s = ret_xf t; globals s = globals t \<rbrakk> \<Longrightarrow> Q s0 s = Q s0' t"
-  shows "\<lbrace>\<lambda>s. P cs \<and> s = globals cs \<and> arg_rel cs \<rbrace>
-           ac_f
-         \<lbrace>\<lambda>r s'. \<exists>cs'. s' = globals cs' \<and> r = ret_xf cs' \<and> Q cs cs' \<rbrace>"
-  apply (clarsimp simp: valid_def ac_def AC_call_L1_def L2_call_L1_def L1_call_simpl_def
-                        in_monad' in_liftM select_f_def in_select in_fail
-                  split: sum.splits xstate.splits)
-  apply (rename_tac r', case_tac r'; clarsimp)
-  apply (rename_tac xst, case_tac xst; clarsimp)
-  apply (drule_tac ?s0.1=s in exec_normal[OF _ _ c_spec[rule_format], rotated])
-   apply (blast dest: precond_deps)
-  apply (blast dest: postcond_deps)
-  done
-
-text \<open>This one is probably more useful\<close>
-lemma autocorres_transfer_spec_no_modifies:
-  assumes ac_def:
-    "ac_f \<equiv> AC_call_L1 arg_rel globals ret_xf (L1_call_simpl check_termination \<Gamma> f_'proc)"
-  assumes c_spec:
-    "\<forall>s0. hoarep \<Gamma> {} {} (P' s0) (Call f_'proc) (Collect (Q s0)) A" -- \<open>syntax parser barfs...\<close>
-  assumes c_modifies:
-    "\<forall>\<sigma>. \<Gamma>\<turnstile>\<^bsub>/UNIV\<^esub> {\<sigma>} Call f_'proc {t. t may_not_modify_globals \<sigma>}"
-  assumes c_spec_unify:
-    "\<And>s0. P' s0 = {s. s0 = s \<and> P s}"
-  assumes precond_deps:
-    "\<And>s0 s t. \<lbrakk> arg_rel s; arg_rel t; globals s = globals t \<rbrakk> \<Longrightarrow> P s = P t"
-  assumes postcond_deps:
-    "\<And>s0 s0' s t. \<lbrakk> arg_rel s0; arg_rel s0'; globals s0 = globals s0';
-                    ret_xf s = ret_xf t; globals s = globals t \<rbrakk> \<Longrightarrow> Q s0 s = Q s0' t"
-  shows "\<lbrace>\<lambda>s. s = globals cs \<and> P cs \<and> arg_rel cs \<rbrace>
-           ac_f
-         \<lbrace>\<lambda>r s'. s' = globals cs \<and> (\<exists>cs'. r = ret_xf cs' \<and> Q cs cs') \<rbrace>"
-  apply (clarsimp simp: valid_def ac_def AC_call_L1_def L2_call_L1_def L1_call_simpl_def
-                        in_monad' in_liftM select_f_def in_select in_fail
-                  split: sum.splits xstate.splits)
-  apply (rename_tac r', case_tac r'; clarsimp)
-  apply (rename_tac xst, case_tac xst; clarsimp)
-  apply (frule_tac ?s0.1=s in exec_normal[OF _ _ c_spec[rule_format], rotated])
-   apply (clarsimp simp: c_spec_unify)
-   apply (blast dest: precond_deps)
-  apply (frule exec_normal[OF singletonI _ c_modifies[rule_format]])
-  apply (clarsimp simp: meq_def)
-  apply (blast dest: postcond_deps)
-  done
-
+text \<open>
+  For wrapped bitfield functions, the @{term hoarep} triples for them can be transferred
+  to @{term valid} triples.
+\<close>
 context kernel_m begin
 
 thm cap_zombie_cap_get_capZombiePtr_spec
@@ -1002,14 +511,18 @@ lemma cap_zombie_cap_get_capZombiePtr'_spec:
   "\<lbrace>\<lambda>s. s = s0 \<and> cap_get_tag cap = scast cap_zombie_cap \<and> get_capZombieBits_CL (cap_zombie_cap_lift cap) < 0x1F\<rbrace>
      cap_zombie_cap_get_capZombiePtr' cap
    \<lbrace>\<lambda>r s. s = s0 \<and> r = get_capZombiePtr_CL (cap_zombie_cap_lift cap)\<rbrace>"
+  (* setup *)
   apply (rule hoare_weaken_pre)
    apply (rule hoare_strengthen_post)
+    (* generic transfer operation *)
     thm autocorres_transfer_spec_no_modifies[OF
           cap_zombie_cap_get_capZombiePtr'_def cap_zombie_cap_get_capZombiePtr_spec]
     apply (rule autocorres_transfer_spec_no_modifies[OF
                   cap_zombie_cap_get_capZombiePtr'_def cap_zombie_cap_get_capZombiePtr_spec _ refl,
                   where cs="undefined\<lparr>globals := s0, cap_' := cap\<rparr>"])
+                        (* the standard tactics can't invent a suitable cs automatically *)
       apply (rule cap_zombie_cap_get_capZombiePtr_modifies)
+     (* prove sanity conditions on local variables and preconds *)
      apply auto
   done
 
@@ -1029,32 +542,22 @@ lemma cap_zombie_cap_get_capZombieType'_spec:
      apply auto
   done
 
-text \<open>Helpers\<close>
-lemma All_to_all':
-  "(\<forall>x. P x) \<Longrightarrow> (\<And>x. P x)"
-  by simp
-text \<open>Convert references to global or local state variables, to the opposite one.
-  FIXME: surely this has been proven already.\<close>
-lemma collect_lift:
-  "Collect (\<lambda>s. s0 = s \<and> f s) = Collect (\<lambda>s. s0 = s \<and> f s0)"
-  by blast
-lemma collect_unlift:
-  "Collect (\<lambda>s. s0 = s \<and> f s0 s) = Collect (\<lambda>s. s0 = s \<and> f s s)"
-  by blast
-
-thm cap_zombie_cap_set_capZombieNumber_spec[THEN All_to_all']
+text \<open>There are some extra complications when transferring bitfield update specs\<close>
+thm cap_zombie_cap_set_capZombieNumber_spec (* extra quantified var; precond talks about initial state *)
 lemma cap_zombie_cap_set_capZombieNumber'_spec:
   "\<lbrace>\<lambda>s. s = s0 \<and> ccap_relation cap' cap \<and> isZombie cap' \<and> capAligned cap' \<and> unat n \<le> zombieCTEs (capZombieType cap')\<rbrace>
      cap_zombie_cap_set_capZombieNumber' cap n
    \<lbrace>\<lambda>r s. s = s0 \<and> ccap_relation (capZombieNumber_update (\<lambda>_. unat n) cap') r\<rbrace>"
   apply (rule hoare_weaken_pre)
    apply (rule hoare_strengthen_post)
+    (* All_to_all' drops the extra quantifier. (rule_format would remove both) *)
     thm autocorres_transfer_spec_no_modifies[OF
           cap_zombie_cap_set_capZombieNumber'_def cap_zombie_cap_set_capZombieNumber_spec[THEN All_to_all']]
     apply (rule autocorres_transfer_spec_no_modifies[OF
                   cap_zombie_cap_set_capZombieNumber'_def cap_zombie_cap_set_capZombieNumber_spec[THEN All_to_all'],
                   where cs="undefined\<lparr>globals := s0, cap_' := cap, n_' := n\<rparr>"])
       apply (rule cap_zombie_cap_set_capZombieNumber_modifies)
+     (* swap initial state var to allow unification *)
      apply (rule collect_unlift)
     apply auto
   done
@@ -1075,54 +578,90 @@ lemma cap_capType_equals'_spec:
      apply auto
   done
 
+(* TODO: any other types of bitfield_gen functions? *)
 
-subsection \<open>Experiment with wrapping specs\<close>
-lemma exec_no_fault:
-  assumes asms: "s \<in> P"
-  and     ce: "Gamma \<turnstile> \<langle>c, Normal s\<rangle> \<Rightarrow> Fault f"
-  and  valid: "Gamma \<turnstile> P c Q, A"
-  shows   "False"
-  using valid ce asms
-  apply -
-  apply (frule hoare_sound)
-  apply (clarsimp simp: NonDetMonad.bind_def cvalid_def split_def HoarePartialDef.valid_def)
-  apply (drule spec, drule spec, drule (1) mp)
-  apply auto
+end
+
+
+
+context kernel_m begin
+text \<open>Termination proofs for use with @{thm ccorres_to_corres_with_termination}. Currently unused.\<close>
+
+lemma cap_get_capType_terminates:
+  "\<Gamma> \<turnstile> Call cap_get_capType_'proc \<down> Normal s"
+  apply (tactic \<open>ALLGOALS (terminates_trivial_tac @{context})\<close>;
+         fail)
   done
 
-lemma exec_no_stuck:
-  assumes asms: "s \<in> P"
-  and     ce: "Gamma \<turnstile> \<langle>c, Normal s\<rangle> \<Rightarrow> Stuck"
-  and  valid: "Gamma \<turnstile> P c Q, A"
-  shows   "False"
-  using valid ce asms
-  apply -
-  apply (frule hoare_sound)
-  apply (clarsimp simp: NonDetMonad.bind_def cvalid_def split_def HoarePartialDef.valid_def)
-  apply (drule spec, drule spec, drule (1) mp)
-  apply auto
+lemma thread_state_get_tcbQueued_terminates:
+  "\<Gamma> \<turnstile> Call thread_state_get_tcbQueued_'proc \<down> Normal s"
+  apply (tactic \<open>ALLGOALS (terminates_trivial_tac @{context})\<close>;
+         fail)
   done
 
-thm clzl_body_def clzl_spec
-
-definition L1_call_simpl_spec where
-  "L1_call_simpl_spec check_term Gamma proc precond postcond =
-     L1_spec (Collect (\<lambda>(s, t). precond s s \<and> postcond s t))"
-
-lemma L1corres_call_simpl_spec:
-  "\<lbrakk> \<forall>s0. Gamma\<turnstile> (Collect (precond s0)) (Call proc) (Collect (postcond s0));
-     \<And>s. ct \<Longrightarrow> Gamma\<turnstile>Call proc \<down> Normal s \<rbrakk> \<Longrightarrow>
-   L1corres ct Gamma (L1_call_simpl_spec ct Gamma proc precond postcond) (Call proc)"
-  apply (clarsimp simp: L1corres_def L1_call_simpl_spec_def L1_defs
-                        assert_def snd_select snd_liftE snd_spec
-                        in_monad' in_spec
-                  split: xstate.splits)
-  apply (case_tac t)
-     apply (blast dest: exec_normal[rotated])
-    apply (blast dest: exec_abrupt[rotated])
-   apply (blast intro: exec_no_fault[rotated])
-  apply (blast intro: exec_no_stuck[rotated])
+lemma thread_state_ptr_set_tcbQueued_terminates:
+  "\<Gamma> \<turnstile> Call thread_state_ptr_set_tcbQueued_'proc \<down> Normal s"
+  apply (tactic \<open>ALLGOALS (terminates_trivial_tac @{context})\<close>;
+         fail)
   done
 
+lemma ready_queues_index_terminates:
+  "\<Gamma> \<turnstile> Call ready_queues_index_'proc \<down> Normal s"
+  apply (tactic \<open>ALLGOALS (terminates_trivial_tac @{context})\<close>;
+         fail)
+  done
+
+lemma prio_to_l1index_terminates:
+  "\<Gamma> \<turnstile> Call prio_to_l1index_'proc \<down> Normal s"
+  apply (tactic \<open>ALLGOALS (terminates_trivial_tac @{context})\<close>;
+         fail)
+  done
+
+lemma removeFromBitmap_terminates:
+  "\<Gamma> \<turnstile> Call removeFromBitmap_'proc \<down> Normal s"
+  apply (tactic \<open>ALLGOALS (terminates_trivial_tac @{context})\<close>;
+         rule prio_to_l1index_terminates)
+  done
+
+lemma addToBitmap_terminates:
+  "\<Gamma> \<turnstile> Call addToBitmap_'proc \<down> Normal s"
+  apply (tactic \<open>ALLGOALS (terminates_trivial_tac @{context})\<close>;
+         rule prio_to_l1index_terminates)
+  done
+
+lemma tcbSchedDequeue_terminates:
+   "\<Gamma> \<turnstile> Call tcbSchedDequeue_'proc \<down> Normal s"
+  apply (tactic \<open>ALLGOALS (terminates_trivial_tac @{context})\<close>;
+         rule thread_state_get_tcbQueued_terminates
+              thread_state_ptr_set_tcbQueued_terminates
+              ready_queues_index_terminates
+              removeFromBitmap_terminates)
+  done
+
+lemma tcbSchedAppend_terminates:
+   "\<Gamma> \<turnstile> Call tcbSchedAppend_'proc \<down> Normal s"
+  apply (tactic \<open>ALLGOALS (terminates_trivial_tac @{context})\<close>;
+         rule thread_state_get_tcbQueued_terminates
+              thread_state_ptr_set_tcbQueued_terminates
+              ready_queues_index_terminates
+              addToBitmap_terminates)
+  done
+
+lemma tcbSchedEnqueue_terminates:
+   "\<Gamma> \<turnstile> Call tcbSchedEnqueue_'proc \<down> Normal s"
+  apply (tactic \<open>ALLGOALS (terminates_trivial_tac @{context})\<close>;
+         rule thread_state_get_tcbQueued_terminates
+              thread_state_ptr_set_tcbQueued_terminates
+              ready_queues_index_terminates
+              addToBitmap_terminates)
+  done
+
+lemma rescheduleRequired_terminates:
+   "\<Gamma> \<turnstile> Call rescheduleRequired_'proc \<down> Normal s"
+  apply (tactic \<open>ALLGOALS (terminates_trivial_tac @{context})\<close>;
+         rule tcbSchedEnqueue_terminates)
+  done
+
+end
 
 end
